Lean4Lean/Verify/Environment/Extension.lean
@@ -1,0 +1,397 @@
+import Lean4Lean.Verify.Environment.Checker
+
+namespace Lean4Lean
+
+open Lean hiding Environment Exception
+open Kernel
+
+open private Lean.Kernel.Environment.add from Lean.Environment
+
+theorem TrEnv.exists_addConst (H : TrEnv safety env venv) (hn : env.find? name = none)
+    (ci' : VConstant) : ∃ venv', venv.addConst name ci' = some venv' := by
+  unfold VEnv.addConst
+  cases hfind : venv.constants name with
+  | none => simp
+  | some ci =>
+    exfalso
+    obtain ⟨ci, hci, _⟩ := H.find?_iff.2 ⟨ci, hfind⟩
+    rw [hn] at hci
+    contradiction
+
+theorem TrEnv'.no_inductInfo (H : TrEnv' .unsafe C Q venv) :
+    C.find? name ≠ some (.inductInfo info) := by
+  induction H with
+  | empty => simp [SMap.find?]
+  | ignore hn hhidden H ih =>
+    rename_i C' Q' env' ci
+    exact False.elim <| hhidden (by cases ci.safety <;> rfl)
+  | «axiom» htr hn hwf hadd H ih =>
+    rw [H.map_wf.find?_insert]
+    split
+    · simp
+    · exact ih
+  | defn htr hn hwf hadd H ih =>
+    rw [H.map_wf.find?_insert]
+    split
+    · simp
+    · exact ih
+  | thm htr hn hwf hprop hadd H ih =>
+    rw [H.map_wf.find?_insert]
+    split
+    · simp
+    · exact ih
+  | «opaque» htr hn hwf hadd H ih =>
+    rw [H.map_wf.find?_insert]
+    split
+    · simp
+    · exact ih
+  | quot hready hadd H ih =>
+    dsimp [AddQuot, AddQuot1] at hadd
+    obtain ⟨lp₁, ty₁, env₁, _, hn₁, _,
+      lp₂, ty₂, env₂, _, hn₂, _,
+      lp₃, ty₃, env₃, _, hn₃, _,
+      lp₄, ty₄, env₄, _, hn₄, _, rfl, _⟩ := hadd
+    have wf₀ := H.map_wf
+    have wf₁ := wf₀.insert ``Quot
+      (.quotInfo { name := ``Quot, kind := .type, levelParams := lp₁, type := ty₁ }) hn₁
+    have wf₂ := wf₁.insert ``Quot.mk
+      (.quotInfo { name := ``Quot.mk, kind := .ctor, levelParams := lp₂, type := ty₂ }) hn₂
+    have wf₃ := wf₂.insert ``Quot.lift
+      (.quotInfo { name := ``Quot.lift, kind := .lift, levelParams := lp₃, type := ty₃ }) hn₃
+    rw [wf₃.find?_insert]
+    split
+    · simp
+    rw [wf₂.find?_insert]
+    split
+    · simp
+    rw [wf₁.find?_insert]
+    split
+    · simp
+    rw [wf₀.find?_insert]
+    split
+    · simp
+    exact ih
+  | induct _ hadd _ _ => exact nomatch hadd
+
+theorem VEnv.addConst_mono {env₁ env₂ env₁' env₂' : VEnv} (H : env₁ ≤ env₂)
+    (h₁ : env₁.addConst name ci = some env₁') (h₂ : env₂.addConst name ci = some env₂') :
+    env₁' ≤ env₂' := by
+  unfold VEnv.addConst at h₁ h₂
+  split at h₁ <;> cases h₁
+  split at h₂ <;> cases h₂
+  constructor
+  · intro n a ha
+    simp at ha ⊢
+    split at ha <;> split <;> simp_all
+    exact H.constants ha
+  · exact H.defeqs
+
+theorem VEnv.addDefEq_mono {env₁ env₂ : VEnv} (H : env₁ ≤ env₂) :
+    env₁.addDefEq df ≤ env₂.addDefEq df := by
+  constructor
+  · exact H.constants
+  · rintro d (rfl | hd)
+    · exact .inl rfl
+    · exact .inr (H.defeqs hd)
+
+theorem VEnv.addConst_eq_of_ne
+    {env env' : VEnv}
+    (hadd : env.addConst name ci = some env') (hne : name ≠ n) :
+    env'.constants n = env.constants n := by
+  unfold VEnv.addConst at hadd
+  split at hadd <;> cases hadd
+  simp [hne]
+
+theorem VEnv.HasPrimitives.addConst {env env' : VEnv} (H : env.HasPrimitives)
+    (hname : Environment.primitives.contains name = false)
+    (hadd : env.addConst name ci = some env') : env'.HasPrimitives := by
+  have le := VEnv.addConst_le hadd
+  have same (n : Name) (hp : Environment.primitives.contains n = true) :
+      env'.constants n = env.constants n :=
+    VEnv.addConst_eq_of_ne hadd fun h => by subst h; simp_all
+  have oldContains (n : Name) (hp : Environment.primitives.contains n = true) :
+      env'.contains n → env.contains n := by
+    rintro ⟨ci, hci⟩
+    exact ⟨ci, (same n hp) ▸ hci⟩
+  have newContains (n : Name) : env.contains n → env'.contains n := by
+    rintro ⟨ci, hci⟩
+    exact ⟨ci, le.constants hci⟩
+  let prims := [
+    ``Bool, ``Bool.false, ``Bool.true,
+    ``Nat, ``Nat.zero, ``Nat.succ,
+    ``Nat.add, ``Nat.pred, ``Nat.sub, ``Nat.mul, ``Nat.pow,
+    ``Nat.gcd, ``Nat.mod, ``Nat.div, ``Nat.beq, ``Nat.ble,
+    ``Nat.bitwise, ``Nat.land, ``Nat.lor, ``Nat.xor,
+    ``Nat.shiftLeft, ``Nat.shiftRight,
+    ``String.ofList, ``Char.ofNat]
+  have hprims : Environment.primitives = .ofList prims := rfl
+  replace hprims {n} : Environment.primitives.contains n ↔ n ∈ prims := by
+    simp [hprims, NameSet.contains, NameSet.ofList]
+  have primBool : Environment.primitives.contains ``Bool = true := hprims.2 (by simp [prims])
+  have primBoolFalse : Environment.primitives.contains ``Bool.false = true :=
+    hprims.2 (by simp [prims])
+  have primBoolTrue : Environment.primitives.contains ``Bool.true = true :=
+    hprims.2 (by simp [prims])
+  have primNat : Environment.primitives.contains ``Nat = true := hprims.2 (by simp [prims])
+  have primNatZero : Environment.primitives.contains ``Nat.zero = true :=
+    hprims.2 (by simp [prims])
+  have primNatSucc : Environment.primitives.contains ``Nat.succ = true :=
+    hprims.2 (by simp [prims])
+  have prim (n : Name) (h : n ∈ [``Nat.add, ``Nat.sub, ``Nat.mul, ``Nat.pow, ``Nat.gcd,
+      ``Nat.mod, ``Nat.div, ``Nat.beq, ``Nat.ble, ``Nat.land, ``Nat.lor, ``Nat.xor,
+      ``Nat.shiftLeft, ``Nat.shiftRight, ``Char.ofNat, ``String.ofList]) :
+      Environment.primitives.contains n = true := by
+    simp at h
+    rcases h with rfl | rfl | rfl | rfl | rfl | rfl | rfl | rfl | rfl | rfl | rfl |
+      rfl | rfl | rfl | rfl | rfl <;> exact hprims.2 (by simp [prims])
+  constructor
+  · intro h
+    let ⟨h1, h2⟩ := H.bool (oldContains _ primBool h)
+    exact ⟨newContains _ h1, newContains _ h2⟩
+  · intro ci h; apply H.boolFalse; rwa [← same _ primBoolFalse]
+  · intro ci h; apply H.boolTrue; rwa [← same _ primBoolTrue]
+  · intro h
+    let ⟨h1, h2⟩ := H.nat (oldContains _ primNat h)
+    exact ⟨newContains _ h1, newContains _ h2⟩
+  · intro ci h; apply H.natZero; rwa [← same _ primNatZero]
+  · intro ci h; apply H.natSucc; rwa [← same _ primNatSucc]
+  · intro h a b; exact (H.natAdd (oldContains _ (prim _ (by simp)) h) a b).mono le
+  · intro h a b; exact (H.natSub (oldContains _ (prim _ (by simp)) h) a b).mono le
+  · intro h a b; exact (H.natMul (oldContains _ (prim _ (by simp)) h) a b).mono le
+  · intro h a b; exact (H.natPow (oldContains _ (prim _ (by simp)) h) a b).mono le
+  · intro h a b; exact (H.natGcd (oldContains _ (prim _ (by simp)) h) a b).mono le
+  · intro h a b; exact (H.natMod (oldContains _ (prim _ (by simp)) h) a b).mono le
+  · intro h a b; exact (H.natDiv (oldContains _ (prim _ (by simp)) h) a b).mono le
+  · intro h a b; exact (H.natBEq (oldContains _ (prim _ (by simp)) h) a b).mono le
+  · intro h a b; exact (H.natBLE (oldContains _ (prim _ (by simp)) h) a b).mono le
+  · intro h a b; exact (H.natLAnd (oldContains _ (prim _ (by simp)) h) a b).mono le
+  · intro h a b; exact (H.natLOr (oldContains _ (prim _ (by simp)) h) a b).mono le
+  · intro h a b; exact (H.natXor (oldContains _ (prim _ (by simp)) h) a b).mono le
+  · intro h a b; exact (H.natShiftLeft (oldContains _ (prim _ (by simp)) h) a b).mono le
+  · intro h a b; exact (H.natShiftRight (oldContains _ (prim _ (by simp)) h) a b).mono le
+  · intro ci h; apply H.charOfNat; rwa [← same _ (prim _ (by simp))]
+  · intro ci h
+    obtain ⟨rfl, h2, h3⟩ := H.stringOfList (by rwa [← same _ (prim _ (by simp))])
+    exact ⟨rfl, h2.mono le, h3.mono le⟩
+
+theorem VEnv.HasPrimitives.addDefEq {env : VEnv} (H : env.HasPrimitives) :
+    (env.addDefEq df).HasPrimitives :=
+  { H with
+    natAdd := fun h a b => (H.natAdd h a b).mono VEnv.addDefEq_le
+    natSub := fun h a b => (H.natSub h a b).mono VEnv.addDefEq_le
+    natMul := fun h a b => (H.natMul h a b).mono VEnv.addDefEq_le
+    natPow := fun h a b => (H.natPow h a b).mono VEnv.addDefEq_le
+    natGcd := fun h a b => (H.natGcd h a b).mono VEnv.addDefEq_le
+    natMod := fun h a b => (H.natMod h a b).mono VEnv.addDefEq_le
+    natDiv := fun h a b => (H.natDiv h a b).mono VEnv.addDefEq_le
+    natBEq := fun h a b => (H.natBEq h a b).mono VEnv.addDefEq_le
+    natBLE := fun h a b => (H.natBLE h a b).mono VEnv.addDefEq_le
+    natLAnd := fun h a b => (H.natLAnd h a b).mono VEnv.addDefEq_le
+    natLOr := fun h a b => (H.natLOr h a b).mono VEnv.addDefEq_le
+    natXor := fun h a b => (H.natXor h a b).mono VEnv.addDefEq_le
+    natShiftLeft := fun h a b => (H.natShiftLeft h a b).mono VEnv.addDefEq_le
+    natShiftRight := fun h a b => (H.natShiftRight h a b).mono VEnv.addDefEq_le
+    stringOfList := fun h =>
+      let ⟨h1, h2, h3⟩ := H.stringOfList h
+      ⟨h1, h2.mono VEnv.addDefEq_le, h3.mono VEnv.addDefEq_le⟩ }
+
+theorem VEnvs.WF.safePrimitives_add {ves : VEnvs} {env : Environment}
+    (wf : ves.WF env) (ci : ConstantInfo)
+    (hfresh : env.find? ci.name = none)
+    (hok : Environment.primitives.contains ci.name →
+      ci.safety = .safe ∧ ci.levelParams = []) :
+    (env.add ci).find? (n : Name) = some (ci' : ConstantInfo) → Environment.primitives.contains n →
+      ci'.safety = .safe ∧ ci'.levelParams = [] := by
+  intro hfind hp
+  have mapWF := (wf.tr (safety := .safe)).map_wf
+  have hnone : env.constants.find? ci.name = none := by
+    rw [← mapWF.find?'_eq_find?]
+    exact hfresh
+  have mapWF' := mapWF.insert ci.name ci hnone
+  change SMap.find?' (env.constants.insert ci.name ci) n = some ci' at hfind
+  rw [mapWF'.find?'_eq_find?, mapWF.find?_insert] at hfind
+  split at hfind
+  · cases hfind
+    rename_i heq
+    have heq' := LawfulBEq.eq_of_beq heq
+    cases heq'
+    exact hok hp
+  · apply wf.safePrimitives ?_ hp
+    rw [Kernel.Environment.find?, mapWF.find?'_eq_find?]
+    exact hfind
+
+theorem addConstCore.WF {env : Environment} {ves : VEnvs} (wf : ves.WF env)
+    (ci : ConstantInfo) (ci' : VConstVal) (checkSafety : DefinitionSafety)
+    (visible_le : ∀ safety, safety ≤ ci.safety → safety ≤ checkSafety)
+    (htr : TrConstVal checkSafety (ves.venv checkSafety) ci ci')
+    (hci : ci'.toVConstant.WF (ves.venv checkSafety))
+    (hn : env.find? ci.name = none)
+    (hprim : Environment.primitives.contains ci.name →
+      ci.safety = .safe ∧ ci.levelParams = [])
+    (preserves : ∀ safety venv', safety ≤ ci.safety →
+      (ves.venv safety).addConst ci.name ci'.toVConstant = some venv' →
+      (ves.venv safety).HasPrimitives → venv'.HasPrimitives)
+    (step : ∀ safety venv',
+      TrConstant safety (ves.venv safety) ci ci'.toVConstant →
+      ci'.toVConstant.WF (ves.venv safety) →
+      (ves.venv safety).addConst ci.name ci'.toVConstant = some venv' →
+      TrEnv' safety env.constants env.quotInit (ves.venv safety) →
+      TrEnv' safety (env.constants.insert ci.name ci) env.quotInit venv') :
+    ∃ ves' : VEnvs, ves'.WF (env.add ci) ∧ ∀ safety, ves.venv safety ≤ ves'.venv safety := by
+  classical
+  have hnMap : env.constants.find? ci.name = none := by
+    rw [← (wf.tr (safety := .safe)).map_wf.find?'_eq_find?]
+    exact hn
+  have visible_tr (safety) (hvisible : safety ≤ ci.safety) :
+      TrConstant safety (ves.venv safety) ci ci'.toVConstant :=
+    (htr.1.sf_mono (visible_le safety hvisible)).mono (wf.mono (visible_le safety hvisible))
+  have visible_wf (safety) (hvisible : safety ≤ ci.safety) :
+      ci'.toVConstant.WF (ves.venv safety) :=
+    hci.mono (wf.mono (visible_le safety hvisible))
+  have hex (safety) (hvisible : safety ≤ ci.safety) :=
+    (wf.tr (safety := safety)).exists_addConst hn ci'.toVConstant
+  let next (safety : DefinitionSafety) : VEnv :=
+    if hvisible : safety ≤ ci.safety then Classical.choose (hex safety hvisible)
+    else ves.venv safety
+  have hadd (safety) (hvisible : safety ≤ ci.safety) :
+      (ves.venv safety).addConst ci.name ci'.toVConstant = some (next safety) := by
+    simpa [next, hvisible] using Classical.choose_spec (hex safety hvisible)
+  let ves' : VEnvs := ⟨next⟩
+  refine ⟨ves', ?_, ?_⟩
+  · refine {
+      tr := ?_
+      hasPrimitives := ?_
+      safePrimitives := wf.safePrimitives_add ci hn hprim
+      mono := ?_ }
+    · intro safety
+      change TrEnv' safety (env.constants.insert ci.name ci) env.quotInit (next safety)
+      by_cases hvisible : safety ≤ ci.safety
+      · exact step safety _ (visible_tr safety hvisible) (visible_wf safety hvisible)
+          (hadd safety hvisible) (wf.tr (safety := safety))
+      · simpa [next, hvisible] using
+          TrEnv'.ignore (ci := ci) hnMap hvisible (wf.tr (safety := safety))
+    · intro safety
+      by_cases hvisible : safety ≤ ci.safety
+      · exact preserves safety _ hvisible (hadd safety hvisible) wf.hasPrimitives
+      · simpa [ves', next, hvisible] using wf.hasPrimitives (safety := safety)
+    · intro safety safety' hle
+      change next safety' ≤ next safety
+      by_cases hvisible' : safety' ≤ ci.safety
+      · have hvisible := DefinitionSafety.le_trans hle hvisible'
+        rw [show next safety' = Classical.choose (hex safety' hvisible') by simp [next, hvisible'],
+          show next safety = Classical.choose (hex safety hvisible) by simp [next, hvisible]]
+        exact VEnv.addConst_mono (wf.mono hle)
+          (Classical.choose_spec (hex safety' hvisible'))
+          (Classical.choose_spec (hex safety hvisible))
+      · rw [show next safety' = ves.venv safety' by simp [next, hvisible']]
+        by_cases hvisible : safety ≤ ci.safety
+        · rw [show next safety = Classical.choose (hex safety hvisible) by simp [next, hvisible]]
+          exact (wf.mono hle).trans
+            (VEnv.addConst_le (Classical.choose_spec (hex safety hvisible)))
+        · rw [show next safety = ves.venv safety by simp [next, hvisible]]
+          exact wf.mono hle
+  · intro safety
+    change ves.venv safety ≤ next safety
+    by_cases hvisible : safety ≤ ci.safety
+    · simpa [next, hvisible] using VEnv.addConst_le (hadd safety hvisible)
+    · simp [next, hvisible, VEnv.LE.rfl]
+
+theorem addConst.WF {env : Environment} {ves : VEnvs} (wf : ves.WF env)
+    (ci : ConstantInfo) (ci' : VConstVal) (checkSafety : DefinitionSafety)
+    (visible_le : ∀ safety, safety ≤ ci.safety → safety ≤ checkSafety)
+    (htr : TrConstVal checkSafety (ves.venv checkSafety) ci ci')
+    (hci : ci'.toVConstant.WF (ves.venv checkSafety))
+    (hn : env.find? ci.name = none)
+    (hnonprim : Environment.primitives.contains ci.name = false)
+    (step : ∀ safety venv',
+      TrConstant safety (ves.venv safety) ci ci'.toVConstant →
+      ci'.toVConstant.WF (ves.venv safety) →
+      (ves.venv safety).addConst ci.name ci'.toVConstant = some venv' →
+      TrEnv' safety env.constants env.quotInit (ves.venv safety) →
+      TrEnv' safety (env.constants.insert ci.name ci) env.quotInit venv') :
+    ∃ ves' : VEnvs, ves'.WF (env.add ci) ∧ ∀ safety, ves.venv safety ≤ ves'.venv safety := by
+  exact addConstCore.WF wf ci ci' checkSafety visible_le htr hci hn
+    (fun hp => by simp_all)
+    (fun _ _ _ hadd hp => hp.addConst hnonprim hadd) step
+
+theorem addDef.WF {env : Environment} {ves : VEnvs} (wf : ves.WF env)
+    (v : DefinitionVal) (ci' : VDefVal) (checkSafety : DefinitionSafety)
+    (visible_le : ∀ safety, safety ≤ (ConstantInfo.defnInfo v).safety → safety ≤ checkSafety)
+    (htr : TrDefVal checkSafety (ves.venv checkSafety) (.defnInfo v) ci')
+    (hci : ci'.WF (ves.venv checkSafety))
+    (hn : env.find? v.name = none)
+    (hprim : Environment.primitives.contains v.name →
+      (ConstantInfo.defnInfo v).safety = .safe ∧ v.levelParams = [])
+    (preserves : ∀ safety base,
+      safety ≤ (ConstantInfo.defnInfo v).safety →
+      (ves.venv safety).addConst v.name ci'.toVConstant = some base →
+      (base.addDefEq ci'.toDefEq).HasPrimitives) :
+    ∃ ves' : VEnvs, ves'.WF (env.add (.defnInfo v)) ∧
+      ∀ safety, ves.venv safety ≤ ves'.venv safety := by
+  classical
+  have hnMap : env.constants.find? v.name = none := by
+    rw [← (wf.tr (safety := .safe)).map_wf.find?'_eq_find?]
+    exact hn
+  have visible_tr (safety) (hvisible : safety ≤ (ConstantInfo.defnInfo v).safety) :
+      TrDefVal safety (ves.venv safety) (.defnInfo v) ci' := by
+    have htr' : TrDefVal safety (ves.venv checkSafety) (.defnInfo v) ci' :=
+      ⟨⟨htr.1.1.sf_mono (visible_le safety hvisible), htr.1.2⟩, htr.2⟩
+    exact htr'.mono (wf.mono (visible_le safety hvisible))
+  have visible_wf (safety) (hvisible : safety ≤ (ConstantInfo.defnInfo v).safety) :
+      ci'.WF (ves.venv safety) := hci.mono (wf.mono (visible_le safety hvisible))
+  have hex (safety) (hvisible : safety ≤ (ConstantInfo.defnInfo v).safety) :=
+    (wf.tr (safety := safety)).exists_addConst hn ci'.toVConstant
+  let base (safety : DefinitionSafety) (hvisible : safety ≤ (ConstantInfo.defnInfo v).safety) :=
+    Classical.choose (hex safety hvisible)
+  let next (safety : DefinitionSafety) : VEnv :=
+    if hvisible : safety ≤ (ConstantInfo.defnInfo v).safety then
+      (base safety hvisible).addDefEq ci'.toDefEq
+    else ves.venv safety
+  have hadd (safety) (hvisible : safety ≤ (ConstantInfo.defnInfo v).safety) :
+      (ves.venv safety).addConst v.name ci'.toVConstant = some (base safety hvisible) :=
+    Classical.choose_spec (hex safety hvisible)
+  let ves' : VEnvs := ⟨next⟩
+  refine ⟨ves', ?_, ?_⟩
+  · refine {
+      tr := ?_
+      hasPrimitives := ?_
+      safePrimitives := wf.safePrimitives_add (.defnInfo v) hn hprim
+      mono := ?_ }
+    · intro safety
+      change TrEnv' safety (env.constants.insert v.name (.defnInfo v)) env.quotInit (next safety)
+      by_cases hvisible : safety ≤ (ConstantInfo.defnInfo v).safety
+      · simpa [next, hvisible] using TrEnv'.defn (visible_tr safety hvisible)
+          (by rwa [← (wf.tr (safety := safety)).map_wf.find?'_eq_find?])
+          (visible_wf safety hvisible) (hadd safety hvisible) (wf.tr (safety := safety))
+      · simpa [next, hvisible, ConstantInfo.name, ConstantInfo.toConstantVal] using
+          TrEnv'.ignore (ci := .defnInfo v) hnMap hvisible (wf.tr (safety := safety))
+    · intro safety
+      by_cases hvisible : safety ≤ (ConstantInfo.defnInfo v).safety
+      · simpa [ves', next, hvisible] using preserves safety (base safety hvisible)
+          hvisible (hadd safety hvisible)
+      · simpa [ves', next, hvisible] using wf.hasPrimitives (safety := safety)
+    · intro safety safety' hle
+      change next safety' ≤ next safety
+      by_cases hvisible' : safety' ≤ (ConstantInfo.defnInfo v).safety
+      · have hvisible := DefinitionSafety.le_trans hle hvisible'
+        rw [show next safety' = (base safety' hvisible').addDefEq ci'.toDefEq by
+              simp [next, hvisible'],
+          show next safety = (base safety hvisible).addDefEq ci'.toDefEq by
+              simp [next, hvisible]]
+        exact VEnv.addDefEq_mono <| VEnv.addConst_mono (wf.mono hle)
+          (hadd safety' hvisible') (hadd safety hvisible)
+      · rw [show next safety' = ves.venv safety' by simp [next, hvisible']]
+        by_cases hvisible : safety ≤ (ConstantInfo.defnInfo v).safety
+        · rw [show next safety = (base safety hvisible).addDefEq ci'.toDefEq by
+              simp [next, hvisible]]
+          exact (wf.mono hle).trans <| (VEnv.addConst_le (hadd safety hvisible)).trans
+            VEnv.addDefEq_le
+        · rw [show next safety = ves.venv safety by simp [next, hvisible]]
+          exact wf.mono hle
+  · intro safety
+    change ves.venv safety ≤ next safety
+    by_cases hvisible : safety ≤ (ConstantInfo.defnInfo v).safety
+    · rw [show next safety = (base safety hvisible).addDefEq ci'.toDefEq by
+          simp [next, hvisible]]
+      exact (VEnv.addConst_le (hadd safety hvisible)).trans VEnv.addDefEq_le
+    · simp [next, hvisible, VEnv.LE.rfl]
